equivalence of algebras `SortedAddMonoidAlgebra` and `AddMonoidAlgebra`

LeanSortedFinsupp/SortedAddMonoidAlgebra.lean
@@ -8,7 +8,7 @@ def SortedAddMonoidAlgebra (R : Type*) [Semiring R] (cmp : G → G → Ordering)
     [Std.LawfulEqCmp cmp] :=
   SortedFinsupp G R cmp
 
-variable (cmp : G → G → Ordering) [Std.TransCmp cmp] [Std.LawfulEqCmp cmp]
+variable {cmp : G → G → Ordering} [Std.TransCmp cmp] [Std.LawfulEqCmp cmp]
 
 section Basic
 
@@ -23,8 +23,42 @@ instance : Zero (SortedAddMonoidAlgebra G R cmp) :=
 instance instFunLike [DecidableEq G] : FunLike (SortedAddMonoidAlgebra G R cmp) G R :=
   inferInstanceAs <| FunLike (SortedFinsupp G R cmp) G R
 
+variable (cmp) in
+def single (x : G) (y : R) [Decidable (y = 0)] : SortedAddMonoidAlgebra G R cmp :=
+  SortedFinsupp.single cmp x y
+
+@[simp]
+lemma single_apply [DecidableEq G] (a : G) (b : R) [Decidable (b = 0)] (c : G) :
+    (single cmp a b) c = if a = c then b else 0 := SortedFinsupp.single_apply ..
+
+@[simp]
+lemma zero_apply [DecidableEq G] (x : G) : (0 : SortedAddMonoidAlgebra G R cmp) x = 0 := rfl
+
+@[simp]
+lemma coe_zero  [DecidableEq G] : ⇑(0 : SortedAddMonoidAlgebra G R cmp) = 0 := rfl
+
+@[simp]
+lemma zero_sum [DecidableEq G] [DecidableEq R]
+    {R' : Type*} [AddCommMonoid R'] (g : G → R → R') :
+    (0 : SortedAddMonoidAlgebra G R cmp).sum g = 0 := rfl
+
+@[simp]
+lemma sum_zero {R' : Type*} [AddCommMonoid R'] [DecidableEq G] [DecidableEq R]
+    (l : SortedAddMonoidAlgebra G R cmp) :
+    l.sum (fun _ _ ↦ 0) = (0 : R') := SortedFinsupp.sum_zero ..
+
+@[ext]
+lemma ext [DecidableEq G] {l1 l2 : SortedAddMonoidAlgebra G R cmp}
+    (h : ∀ s : G, l1 s = l2 s) :
+  l1 = l2 := SortedFinsupp.ext h
+
 instance instAdd [(a : R) → Decidable (a = 0)] :
     Add (SortedAddMonoidAlgebra G R cmp) := SortedFinsupp.instAdd
+
+@[simp]
+lemma add_apply [DecidableEq G] [(a : R) → Decidable (a = 0)]
+    (l₁ l₂ : SortedAddMonoidAlgebra G R cmp) (x : G) :
+    (l₁ + l₂) x = l₁ x + l₂ x := SortedFinsupp.add_apply ..
 
 instance instAddMonoid [(a : R) → Decidable (a = 0)] [DecidableEq G] :
     AddMonoid (SortedAddMonoidAlgebra G R cmp) :=
@@ -34,16 +68,42 @@ instance instAddCommMonoid [(a : R) → Decidable (a = 0)] [DecidableEq G] :
     AddCommMonoid (SortedAddMonoidAlgebra G R cmp) :=
   inferInstanceAs <| AddCommMonoid (SortedFinsupp G R cmp)
 
-instance instSMulWithZero {M} [Zero M] [SMulWithZero M R] [∀ y : R, Decidable (y = 0)] :
+instance instSMulWithZero {M} [Zero M] [SMulWithZero M R]
+    [∀ y : R, Decidable (y = 0)] :
     SMulWithZero M (SortedAddMonoidAlgebra G R cmp) :=
   inferInstanceAs <| SMulWithZero M (SortedFinsupp G R cmp)
+
+instance instSMul {M} [Zero M] [SMulWithZero M R] [∀ y : R, Decidable (y = 0)] :
+    SMul M (SortedAddMonoidAlgebra G R cmp) := inferInstance
 
 lemma smul_def {M} [Zero M] [SMulWithZero M R] [∀ y : R, Decidable (y = 0)]
     (s : M) (l : SortedAddMonoidAlgebra G R cmp) :
     s • l = l.mapRange (fun _ ↦ (s • ·)) (by simp) := rfl
 
-end Basic
+@[simp]
+lemma smul_apply [DecidableEq G] {M} [Zero M] [SMulWithZero M R] [∀ y : R, Decidable (y = 0)]
+    (s : M) (l : SortedAddMonoidAlgebra G R cmp) (x : G) :
+    (s • l) x = s • (l x) := SortedFinsupp.smul_apply ..
 
+def addEquivAddMonoidAlgebra [(a : R) → Decidable (a = 0)] [DecidableEq G] :
+    AddEquiv (SortedAddMonoidAlgebra G R cmp) (AddMonoidAlgebra R G) :=
+  SortedFinsupp.addEquivFinsupp
+
+@[simp]
+lemma addEquivAddMonoidAlgebra_apply [(a : R) → Decidable (a = 0)] [DecidableEq G]
+    (l : SortedAddMonoidAlgebra G R cmp) (x : G) :
+    addEquivAddMonoidAlgebra l x = l x := SortedFinsupp.equivFinsupp_apply ..
+
+lemma addEquivAddMonoidAlgebra_zero [(a : R) → Decidable (a = 0)] [DecidableEq G] :
+    addEquivAddMonoidAlgebra (0 : SortedAddMonoidAlgebra G R cmp) = 0 := rfl
+
+def singleAddHom [DecidableEq G] [∀ i : R, Decidable (i = 0)] (x : G) :
+    R →+ SortedAddMonoidAlgebra G R cmp := {
+  SortedFinsupp.singleAddHom x with
+  toFun y := single cmp x y
+}
+
+end Basic
 section Mul
 
 variable {R} [Semiring R] [AddCommMonoid G] [DecidableEq G] [DecidableEq R]
@@ -76,11 +136,94 @@ lemma mul_apply (l₁ l₂ : SortedAddMonoidAlgebra G R cmp) (x : G) :
   · simp [h]
   · simp [h]
 
-#check SkewMonoidAlgebra.mapDomain
+lemma addEquivAddMonoidAlgebra_mul
+    (l₁ l₂ : SortedAddMonoidAlgebra G R cmp) :
+    addEquivAddMonoidAlgebra (l₁ * l₂) =
+      addEquivAddMonoidAlgebra l₁ * addEquivAddMonoidAlgebra l₂ := by
+  ext
+  simp [mul_apply, AddMonoidAlgebra.mul_apply, Finsupp.sum.eq_def,
+    SortedFinsupp.sum_eq_sum_support]
+  rfl
 
-lemma equivFinsupp_mul (l₁ l₂ : SortedAddMonoidAlgebra G R cmp) (x : G) :
-    (l₁ * l₂) x = l₁.sum fun a₁ b₁ => l₂.sum fun a₂ b₂ => if a₁ + a₂ = x then b₁ * b₂ else 0 := by
-  rw [mul_apply]
+
+def ringEquivAddMonoidAlgebra :
+    RingEquiv (SortedAddMonoidAlgebra G R cmp) (AddMonoidAlgebra R G) := {
+    addEquivAddMonoidAlgebra with
+    map_mul' := addEquivAddMonoidAlgebra_mul
+  }
+
+
+lemma mul_eq (l₁ l₂ : SortedAddMonoidAlgebra G R cmp) : l₁ * l₂ =
+    addEquivAddMonoidAlgebra.symm (addEquivAddMonoidAlgebra l₁ * addEquivAddMonoidAlgebra l₂) := by
+  simp [← addEquivAddMonoidAlgebra_mul]
+
+instance instSemiring : Semiring (SortedAddMonoidAlgebra G R cmp) where
+  left_distrib a b c := by simp [mul_eq, mul_add]
+  right_distrib a b c := by simp [mul_eq, add_mul]
+  zero_mul := by simp [ext_iff, mul_apply]
+  mul_zero := by simp [ext_iff, mul_apply]
+  mul_assoc := by simp [mul_eq, mul_assoc]
+  one := single cmp 0 1
+  one_mul := by
+    convert_to ∀ (a : SortedAddMonoidAlgebra G R cmp), single cmp 0 (1 : R) * a = a
+    simp [ext_iff, mul_apply, single]
+    simp [SortedFinsupp.sum_eq_sum_support, SortedFinsupp.mem_support_iff]
+    simp_intro ..
+  mul_one := by
+    convert_to ∀ (a : SortedAddMonoidAlgebra G R cmp), a * single cmp 0 (1 : R) = a
+    simp [ext_iff, mul_apply, single]
+    simp [SortedFinsupp.sum_eq_sum_support, SortedFinsupp.mem_support_iff]
+    simp_intro ..
+
+instance instCommSemiring {R} [CommSemiring R] [DecidableEq R] :
+    CommSemiring (SortedAddMonoidAlgebra G R cmp) where
+  mul_comm := by simp [mul_eq, mul_comm]
+
+#check AddMonoidAlgebra.singleZeroAlgHom
+def singleZeroRingHom {R} [DecidableEq R] [Semiring R] :
+    R →+* SortedAddMonoidAlgebra G R cmp :=
+  { singleAddHom 0 with
+    map_one' := rfl
+    map_mul' _ _ := by
+      ext
+      simp [singleAddHom, mul_apply, single]
+      -- why `simp` and `simp_rw` doesn't work here?
+      rw [SortedFinsupp.single_apply]
+    }
+
+end Mul
+
+section Algebra
+
+variable [AddCommMonoid G]
+variable {R : Type*} {M} [CommSemiring R] [CommSemiring M] [Algebra M R]
+variable [fact : Fact <| ∀ (a i j : G), cmp i j = cmp (a + i) (a + j)]
+variable [DecidableEq G] [DecidableEq R]
+
+-- def
+#check AddMonoidAlgebra.singleZeroAlgHom
+instance : Algebra M (SortedAddMonoidAlgebra G R cmp) where
+  algebraMap := singleZeroRingHom.comp (algebraMap M R)
+  commutes' _ _ := mul_comm ..
+  smul_def' r x := by
+    ext
+    simp [singleZeroRingHom, singleAddHom, mul_apply, single,
+      SortedFinsupp.sum_eq_sum_support, Algebra.smul_def]
+    split_ifs with h
+    · simp [h]
+    · simp [SortedFinsupp.mem_support_iff]
+      simp_intro _
+
+def algEquivAddMonoidAlgebra [DecidableEq G] :
+    (SortedAddMonoidAlgebra G R cmp) ≃ₐ[M] (AddMonoidAlgebra R G) := {
+    ringEquivAddMonoidAlgebra with
+    commutes' r := by
+      simp [ringEquivAddMonoidAlgebra]
+      ext x
+      simp [AddMonoidAlgebra.single_apply]
+      convert_to (single cmp 0 (algebraMap M R r) : SortedAddMonoidAlgebra G R cmp) x = _
+      simp
+  }
 
 #check AddMonoidAlgebra.mul_apply
 
@@ -91,12 +234,22 @@ lemma equivFinsupp_mul (l₁ l₂ : SortedAddMonoidAlgebra G R cmp) (x : G) :
 #check AddMonoidAlgebra.domCongr
 #check AddMonoidAlgebra.algebra
 #check AddMonoidAlgebra.commSemiring
+#check AddMonoidAlgebra.semiring
 #check Finsupp.instAddCommMonoid
 #check Submodule
 #check AddMonoidAlgebra.mul_def
 
-end Mul
+end Algebra
 
+section Semiring
+
+variable {R} [Semiring R] [AddCommMonoid G] [DecidableEq G] [DecidableEq R]
+variable [fact : Fact <| ∀ (a i j : G), cmp i j = cmp (a + i) (a + j)]
+variable (l₁ l₂ : SortedAddMonoidAlgebra G R cmp)
+
+#synth Mul (SortedAddMonoidAlgebra G R cmp)
+
+end Semiring
 
 -- variable {M} [Zero M] [SMulWithZero R M]
 -- instance algebra {R k G} [CommSemiring R] [Semiring k] [Algebra R k] [AddMonoid G] :
